added useful lemmas and closed the expr case of interp

Pullback/SSA/Basic.lean
@@ -111,9 +111,9 @@ Fin.last' - Fin.cast (size_reverse) res) (as.reverse.findFinIdx? p)
 def Map.get {α β} [DecidableEq α] (map : Map α β) (key : α) : Option β :=
     map.findLast? (·.1 = key) |>.map (·.2)
 
-def Map.uniqueKeys {α β} [DecidableEq α] (x : Map α β) := (x.toList.map (·.1)).Nodup
-
 def Map.keys {α β} [DecidableEq α] (x : Map α β) := x.map (·.1)
+
+def Map.uniqueKeys {α β} [DecidableEq α] (x : Map α β) := (x.keys.toList).Nodup
 
 def Map.keysEq {α β} [DecidableEq α] (x y : Map α β) := x.keys = y.keys
 
